rename MemLog to Log

src/ExampleMemLog.v
@@ -4,7 +4,7 @@ Require Import Hoare.
 Require Import Word.
 Require Import SepAuto.
 Require Import BasicProg.
-Require Import MemLog.
+Require Import Log.
 Require Import Bool.
 Require Import GenSep.
 Require Import Idempotent.
@@ -36,31 +36,31 @@ Proof.
 Qed.
 
 Definition log_inc_two_body T xp s0 s1 mscs rx : prog T :=
-  let^ (mscs, v0) <- MEMLOG.read xp s0 mscs;
-  mscs <- MEMLOG.write xp s0 (v0 ^+ $1) mscs;
-  let^ (mscs, v1) <- MEMLOG.read xp s1 mscs;
-  mscs <- MEMLOG.write xp s1 (v1 ^+ $1) mscs;
+  let^ (mscs, v0) <- LOG.read xp s0 mscs;
+  mscs <- LOG.write xp s0 (v0 ^+ $1) mscs;
+  let^ (mscs, v1) <- LOG.read xp s1 mscs;
+  mscs <- LOG.write xp s1 (v1 ^+ $1) mscs;
   rx mscs.
 
 Theorem log_inc_two_body_ok: forall xp s0 s1 mscs,
   {< mbase m v0 v1 F Fm,
-  PRE             MEMLOG.rep xp Fm (ActiveTxn mbase m) mscs * 
+  PRE             LOG.rep xp Fm (ActiveTxn mbase m) mscs * 
                   [[ (s0 |-> v0 * s1 |-> v1 * F)%pred (list2mem m)]]
-  POST RET:mscs   exists m', MEMLOG.rep xp Fm (ActiveTxn mbase m') mscs *
+  POST RET:mscs   exists m', LOG.rep xp Fm (ActiveTxn mbase m') mscs *
                   [[ (s0 |-> (v0 ^+ $1) * s1 |-> (v1 ^+ $1) * F)%pred (list2mem m') ]]
-  CRASH           MEMLOG.would_recover_old xp Fm mbase
+  CRASH           LOG.would_recover_old xp Fm mbase
   >} log_inc_two_body xp s0 s1 mscs.
 Proof.
   unfold log_inc_two_body.
-  hoare; apply MEMLOG.activetxn_would_recover_old.
+  hoare; apply LOG.activetxn_would_recover_old.
 Qed.
 
 Hint Extern 1 ({{_}} progseq (log_inc_two_body _ _ _ _) _) => apply log_inc_two_body_ok : prog.
 
 Definition log_inc_two T xp s0 s1 cs rx : prog T :=
-  mscs <- MEMLOG.begin xp cs;
+  mscs <- LOG.begin xp cs;
   mscs <- log_inc_two_body xp s0 s1 mscs;
-  let^ (mscs, ok) <- MEMLOG.commit xp mscs;
+  let^ (mscs, ok) <- LOG.commit xp mscs;
   If (bool_dec ok true) {
     rx ^(mscs, ok)
   } else {
@@ -69,22 +69,22 @@ Definition log_inc_two T xp s0 s1 cs rx : prog T :=
 
 Theorem log_inc_two_ok: forall xp s0 s1 mscs,
   {< mbase v0 v1 F Fm,
-  PRE             MEMLOG.rep xp Fm (NoTransaction mbase) mscs * 
+  PRE             LOG.rep xp Fm (NoTransaction mbase) mscs * 
                   [[ (s0 |-> v0 * s1 |-> v1 * F)%pred (list2mem mbase)]]
   POST RET:^(mscs, r)
-                  [[ r = false ]] * MEMLOG.rep xp Fm (NoTransaction mbase) mscs \/
-                  [[ r = true ]] * exists m', MEMLOG.rep xp Fm (NoTransaction m') mscs *
+                  [[ r = false ]] * LOG.rep xp Fm (NoTransaction mbase) mscs \/
+                  [[ r = true ]] * exists m', LOG.rep xp Fm (NoTransaction m') mscs *
                   [[ (s0 |-> (v0 ^+ $1) * s1 |-> (v1 ^+ $1) * F)%pred (list2mem m') ]]
-  CRASH           MEMLOG.would_recover_old xp Fm mbase \/
-                  exists m', MEMLOG.would_recover_either xp Fm mbase m' *
+  CRASH           LOG.would_recover_old xp Fm mbase \/
+                  exists m', LOG.would_recover_either xp Fm mbase m' *
                   [[ (s0 |-> (v0 ^+ $1) * s1 |-> (v1 ^+ $1) * F)%pred (list2mem m') ]]
   >} log_inc_two xp s0 s1 mscs.
 Proof.
   unfold log_inc_two.
   hoare.
-  rewrite MEMLOG.notxn_would_recover_old.
+  rewrite LOG.notxn_would_recover_old.
   cancel.
-  rewrite MEMLOG.activetxn_would_recover_old.
+  rewrite LOG.activetxn_would_recover_old.
   cancel.
 Qed.
 
@@ -97,17 +97,17 @@ Definition i2 xp s0 s1 T := @log_inc_two T xp s0 s1.
 Theorem log_inc_two_recover_ok: forall xp s0 s1 mscs,
   {<< v0 v1 F Fm mbase,
   PRE
-    MEMLOG.rep xp Fm (NoTransaction mbase) mscs *
+    LOG.rep xp Fm (NoTransaction mbase) mscs *
     [[ (s0 |-> v0 * s1 |-> v1 * F)%pred (list2mem mbase)]]
   POST RET:^(mscs, r)
-    [[ r = false ]] * MEMLOG.rep xp Fm (NoTransaction mbase) mscs \/
-    [[ r = true ]] * exists m', MEMLOG.rep xp Fm (NoTransaction m') mscs *
+    [[ r = false ]] * LOG.rep xp Fm (NoTransaction mbase) mscs \/
+    [[ r = true ]] * exists m', LOG.rep xp Fm (NoTransaction m') mscs *
     [[ (s0 |-> (v0 ^+ $1) * s1 |-> (v1 ^+ $1) * F)%pred (list2mem m') ]]
   REC RET:^(mscs, xp)
-    MEMLOG.rep xp Fm (NoTransaction mbase) mscs \/
-    exists m', MEMLOG.rep xp Fm (NoTransaction m') mscs *
+    LOG.rep xp Fm (NoTransaction mbase) mscs \/
+    exists m', LOG.rep xp Fm (NoTransaction m') mscs *
                [[ (s0 |-> (v0 ^+ $1) * s1 |-> (v1 ^+ $1) * F)%pred (list2mem m') ]]
-  >>} log_inc_two xp s0 s1 mscs >> MEMLOG.recover.
+  >>} log_inc_two xp s0 s1 mscs >> LOG.recover.
 Proof.
   intros.
   unfold forall_helper at 1 2; intros v0 v1 F.
@@ -115,7 +115,7 @@ Proof.
   eapply pimpl_ok3.
   eapply corr3_from_corr2_rx; eauto with prog.
   
-  eapply (MEMLOG.recover_corr2_to_corr3 (i2 xp s0 s1)).
+  eapply (LOG.recover_corr2_to_corr3 (i2 xp s0 s1)).
   unfold i2.
   intros.
   eapply pimpl_ok2.
