src/BFileRec.v
@@ -1,5 +1,5 @@
 Require Import Eqdep_dec Arith Omega List.
-Require Import Word WordAuto Pred GenSep Rec Prog BasicProg Hoare SepAuto Array MemLog.
+Require Import Word WordAuto Pred GenSep Rec Prog BasicProg Hoare SepAuto Array Log.
 Require Import BFile RecArray Inode.
 Require Import GenSep.
 Require Import GenSepN.
@@ -218,7 +218,7 @@ Section RECBFILE.
 
   Theorem bf_get_pair_ok : forall lxp bxp ixp inum mscs block_ix pos,
     {< F F1 A mbase m flist f ilistlist,
-    PRE    MEMLOG.rep lxp F (ActiveTxn mbase m) mscs *
+    PRE    LOG.rep lxp F (ActiveTxn mbase m) mscs *
            [[ (F1 * BFILE.rep bxp ixp flist)%pred (list2mem m) ]] *
            [[ (A * # inum |-> f)%pred (list2nmem flist) ]] *
            [[ array_item_pairs ilistlist (list2nmem (BFILE.BFData f)) ]] *
@@ -226,9 +226,9 @@ Section RECBFILE.
            [[ wordToNat block_ix < length (BFILE.BFData f) ]] *
            [[ (pos < items_per_valu)%word ]]
     POST RET:^(mscs,r)
-           MEMLOG.rep lxp F (ActiveTxn mbase m) mscs *
+           LOG.rep lxp F (ActiveTxn mbase m) mscs *
            [[ r = sel (sel ilistlist block_ix nil) pos item_zero ]]
-    CRASH  MEMLOG.would_recover_old lxp F mbase
+    CRASH  LOG.would_recover_old lxp F mbase
     >} bf_get_pair lxp ixp inum block_ix pos mscs.
   Proof.
     unfold bf_get_pair.
@@ -248,7 +248,7 @@ Section RECBFILE.
 
   Theorem bf_put_pair_ok : forall lxp bxp ixp inum mscs block_ix pos i,
     {< F F1 A mbase m flist f ilistlist,
-    PRE      MEMLOG.rep lxp F (ActiveTxn mbase m) mscs *
+    PRE      LOG.rep lxp F (ActiveTxn mbase m) mscs *
              [[ (F1 * BFILE.rep bxp ixp flist)%pred (list2mem m) ]] *
              [[ (A * # inum |-> f)%pred (list2nmem flist) ]] *
              [[ array_item_pairs ilistlist (list2nmem (BFILE.BFData f)) ]] *
@@ -258,13 +258,13 @@ Section RECBFILE.
              [[ Rec.well_formed i ]]
     POST RET:mscs
              exists m' flist' f',
-             MEMLOG.rep lxp F (ActiveTxn mbase m') mscs *
+             LOG.rep lxp F (ActiveTxn mbase m') mscs *
              [[ (F1 * BFILE.rep bxp ixp flist')%pred (list2mem m') ]] *
              [[ (A * # inum |-> f')%pred (list2nmem flist') ]] *
              [[ array_item_pairs (upd ilistlist block_ix 
                                      (upd (sel ilistlist block_ix nil) pos i))
                                  (list2nmem (BFILE.BFData f')) ]]
-    CRASH    MEMLOG.would_recover_old lxp F mbase
+    CRASH    LOG.would_recover_old lxp F mbase
     >} bf_put_pair lxp ixp inum block_ix pos i mscs.
   Proof.
     unfold bf_put_pair.
@@ -536,14 +536,14 @@ Section RECBFILE.
 
   Theorem bf_getlen_ok : forall lxp bxp ixp inum mscs,
     {< F F1 A mbase m flist f ilist,
-    PRE    MEMLOG.rep lxp F (ActiveTxn mbase m) mscs *
+    PRE    LOG.rep lxp F (ActiveTxn mbase m) mscs *
            [[ array_item_file f ilist ]] *
            [[ (F1 * BFILE.rep bxp ixp flist)%pred (list2mem m) ]] *
            [[ (A * #inum |-> f)%pred (list2nmem flist) ]]
     POST RET:^(mscs,r)
-           MEMLOG.rep lxp F (ActiveTxn mbase m) mscs *
+           LOG.rep lxp F (ActiveTxn mbase m) mscs *
            [[ r = $ (length ilist) ]]
-    CRASH  MEMLOG.would_recover_old lxp F mbase
+    CRASH  LOG.would_recover_old lxp F mbase
     >} bf_getlen lxp ixp inum mscs.
   Proof.
     unfold bf_getlen.
@@ -556,15 +556,15 @@ Section RECBFILE.
 
   Theorem bf_get_ok : forall lxp bxp ixp inum idx mscs,
     {< F F1 A mbase m flist f ilist,
-    PRE    MEMLOG.rep lxp F (ActiveTxn mbase m) mscs *
+    PRE    LOG.rep lxp F (ActiveTxn mbase m) mscs *
            [[ array_item_file f ilist ]] *
            [[ (F1 * BFILE.rep bxp ixp flist)%pred (list2mem m) ]] *
            [[ (A * #inum |-> f)%pred (list2nmem flist) ]] *
            [[ wordToNat idx < length ilist ]]
     POST RET:^(mscs,r)
-           MEMLOG.rep lxp F (ActiveTxn mbase m) mscs *
+           LOG.rep lxp F (ActiveTxn mbase m) mscs *
            [[ r = sel ilist idx item_zero ]]
-    CRASH  MEMLOG.would_recover_old lxp F mbase
+    CRASH  LOG.would_recover_old lxp F mbase
     >} bf_get lxp ixp inum idx mscs.
   Proof.
     unfold bf_get.
@@ -584,7 +584,7 @@ Section RECBFILE.
 
   Theorem bf_put_ok : forall lxp bxp ixp inum idx v mscs,
     {< F F1 A mbase m flist f ilist,
-    PRE      MEMLOG.rep lxp F (ActiveTxn mbase m) mscs *
+    PRE      LOG.rep lxp F (ActiveTxn mbase m) mscs *
              [[ array_item_file f ilist ]] *
              [[ (F1 * BFILE.rep bxp ixp flist)%pred (list2mem m) ]] *
              [[ (A * #inum |-> f)%pred (list2nmem flist) ]] *
@@ -592,11 +592,11 @@ Section RECBFILE.
              [[ Rec.well_formed v ]]
     POST RET:mscs
              exists m' flist' f',
-             MEMLOG.rep lxp F (ActiveTxn mbase m') mscs *
+             LOG.rep lxp F (ActiveTxn mbase m') mscs *
              [[ array_item_file f' (upd ilist idx v) ]] *
              [[ (F1 * BFILE.rep bxp ixp flist')%pred (list2mem m') ]] *
              [[ (A * #inum |-> f')%pred (list2nmem flist') ]]
-    CRASH  MEMLOG.would_recover_old lxp F mbase
+    CRASH  LOG.would_recover_old lxp F mbase
     >} bf_put lxp ixp inum idx v mscs.
   Proof.
     unfold bf_put.
@@ -617,19 +617,19 @@ Section RECBFILE.
 
   Theorem bf_extend_ok : forall lxp bxp ixp inum v mscs,
     {< F F1 A mbase m flist f ilist,
-    PRE   MEMLOG.rep lxp F (ActiveTxn mbase m) mscs *
+    PRE   LOG.rep lxp F (ActiveTxn mbase m) mscs *
           [[ array_item_file f ilist ]] *
           [[ (F1 * BFILE.rep bxp ixp flist)%pred (list2mem m) ]] *
           [[ (A * #inum |-> f)%pred (list2nmem flist) ]] *
           [[ Rec.well_formed v ]]
     POST RET:^(mscs, r)
-          exists m', MEMLOG.rep lxp F (ActiveTxn mbase m') mscs *
+          exists m', LOG.rep lxp F (ActiveTxn mbase m') mscs *
           ([[ r = false ]] \/
            [[ r = true ]] * exists flist' f',
            [[ array_item_file f' (ilist ++ (upd item0_list $0 v)) ]] *
            [[ (F1 * BFILE.rep bxp ixp flist')%pred (list2mem m') ]] *
            [[ (A * #inum |-> f')%pred (list2nmem flist') ]] )
-    CRASH  MEMLOG.would_recover_old lxp F mbase
+    CRASH  LOG.would_recover_old lxp F mbase
     >} bf_extend lxp bxp ixp inum v mscs.
   Proof.
     unfold bf_extend.
