src/Testprog.v
@@ -1,5 +1,5 @@
 Require Import Prog.
-Require Import MemLog.
+Require Import Log.
 Require Import Word.
 Require Import Balloc.
 Require Import BFile.
@@ -12,8 +12,8 @@ Set Implicit Arguments.
 
 
 Definition copy_block T xp (a b : addr) mscs rx : prog T :=
-  let^ (mscs, v) <- MEMLOG.read xp a mscs;
-  mscs <- MEMLOG.write xp b v mscs;
+  let^ (mscs, v) <- LOG.read xp a mscs;
+  mscs <- LOG.write xp b v mscs;
   rx mscs.
 
 Fixpoint copy_many T xp (count : nat) (src dst : addr) mscs rx : prog T :=
@@ -27,45 +27,45 @@ Fixpoint copy_many T xp (count : nat) (src dst : addr) mscs rx : prog T :=
 
 Definition testcopy T xp rx : prog T :=
   cs <- BUFCACHE.init 1000 ;
-  mscs <- MEMLOG.init xp cs ;
-  mscs <- MEMLOG.begin xp mscs ;
+  mscs <- LOG.init xp cs ;
+  mscs <- LOG.begin xp mscs ;
   mscs <- copy_many xp 200 $100 $500 mscs ;
-  let^ (mscs, ok) <- MEMLOG.commit xp mscs ;
+  let^ (mscs, ok) <- LOG.commit xp mscs ;
   rx ok.
 
 Definition testalloc T lxp bxp rx : prog T :=
   cs <- BUFCACHE.init 1000 ;
-  mscs <- MEMLOG.init lxp cs ;
-  mscs <- MEMLOG.begin lxp mscs ;
+  mscs <- LOG.init lxp cs ;
+  mscs <- LOG.begin lxp mscs ;
   let^ (mscs, b) <- BALLOC.alloc lxp bxp mscs ;
   match b with
   | None =>
-    mscs <- MEMLOG.abort lxp mscs ;
+    mscs <- LOG.abort lxp mscs ;
     rx None
   | Some bn =>
-    mscs <- MEMLOG.write lxp $0 (addr2valu bn) mscs ;
-    let^ (mscs, ok) <- MEMLOG.commit lxp mscs ;
+    mscs <- LOG.write lxp $0 (addr2valu bn) mscs ;
+    let^ (mscs, ok) <- LOG.commit lxp mscs ;
     rx (Some bn)
   end.
 
 Definition test_bfile T fsxp v mscs rx : prog T :=
-  mscs <- MEMLOG.begin (FSXPMemLog fsxp) mscs ;
-  let^ (mscs, ok) <- BFILE.bfgrow (FSXPMemLog fsxp) (FSXPBlockAlloc fsxp) (FSXPInode fsxp) $3 mscs ;
+  mscs <- LOG.begin (FSXPLog fsxp) mscs ;
+  let^ (mscs, ok) <- BFILE.bfgrow (FSXPLog fsxp) (FSXPBlockAlloc fsxp) (FSXPInode fsxp) $3 mscs ;
   match ok with
   | false =>
-    mscs <- MEMLOG.abort (FSXPMemLog fsxp) mscs ;
+    mscs <- LOG.abort (FSXPLog fsxp) mscs ;
     rx ^(mscs, None)
   | true =>
-    mscs <- BFILE.bfwrite (FSXPMemLog fsxp) (FSXPInode fsxp) $3 $0 v mscs ;
-    let^ (mscs, ok) <- MEMLOG.commit (FSXPMemLog fsxp) mscs ;
+    mscs <- BFILE.bfwrite (FSXPLog fsxp) (FSXPInode fsxp) $3 $0 v mscs ;
+    let^ (mscs, ok) <- LOG.commit (FSXPLog fsxp) mscs ;
 
     match ok with
     | false => rx ^(mscs, None)
     | true =>
-      mscs <- MEMLOG.begin (FSXPMemLog fsxp) mscs ;
-      let^ (mscs, b) <- BFILE.bfread (FSXPMemLog fsxp) (FSXPInode fsxp) $3 $0 mscs ;
-      mscs <- BFILE.bfshrink (FSXPMemLog fsxp) (FSXPBlockAlloc fsxp) (FSXPInode fsxp) $3 mscs ;
-      let^ (mscs, ok) <- MEMLOG.commit (FSXPMemLog fsxp) mscs ;
+      mscs <- LOG.begin (FSXPLog fsxp) mscs ;
+      let^ (mscs, b) <- BFILE.bfread (FSXPLog fsxp) (FSXPInode fsxp) $3 $0 mscs ;
+      mscs <- BFILE.bfshrink (FSXPLog fsxp) (FSXPBlockAlloc fsxp) (FSXPInode fsxp) $3 mscs ;
+      let^ (mscs, ok) <- LOG.commit (FSXPLog fsxp) mscs ;
       match ok with
       | false => rx ^(mscs, None)
       | true => rx ^(mscs, Some b)
@@ -74,7 +74,7 @@ Definition test_bfile T fsxp v mscs rx : prog T :=
   end.
 
 Definition test_bfile_bulkwrite T fsxp v nblocks mscs rx : prog T :=
-  mscs <- MEMLOG.begin (FSXPMemLog fsxp) mscs;
+  mscs <- LOG.begin (FSXPLog fsxp) mscs;
   let^ (mscs) <- For block < nblocks
     Ghost [ (_:unit) ]
     Loopvar [ mscs ]
@@ -82,10 +82,10 @@ Definition test_bfile_bulkwrite T fsxp v nblocks mscs rx : prog T :=
     Invariant emp
     OnCrash emp
     Begin
-      mscs <- BFILE.bfwrite (FSXPMemLog fsxp) (FSXPInode fsxp) $3 block v mscs;
+      mscs <- BFILE.bfwrite (FSXPLog fsxp) (FSXPInode fsxp) $3 block v mscs;
       lrx ^(mscs)
   Rof ^(mscs);
-  let^ (mscs, ok) <- MEMLOG.commit (FSXPMemLog fsxp) mscs;
+  let^ (mscs, ok) <- LOG.commit (FSXPLog fsxp) mscs;
   rx ^(mscs, ok).
 
 (* Why does this seemingly simple function take forever to compile?? *)
